Struggling...

lib/Any.v
@@ -1,4 +1,5 @@
 Require Import Coqlib.
+Require Import Coq.Logic.IndefiniteDescription.
 
 Set Implicit Arguments.
 
@@ -10,6 +11,7 @@ Module Type ANY.
   Parameter val: forall (a: t), (ty a).
   Parameter upcast: forall {T: Type}, T -> t.
   Parameter downcast: forall {T: Type}, t -> option T.
+  (* Parameter downcast_fst: forall {T: Type}, t -> option (T * t). *)
 
   Parameter upcast_inj: forall A B (a: A) (b: B) (EQ: upcast a = upcast b),
       <<EQ: A = B>> /\ <<EQ: a ~= b>>.
@@ -21,6 +23,7 @@ Module Type ANY.
   Parameter downcast_intro: forall (a: t) T (v: T) (TY: (ty a) = T) (VAL: (val a) ~= v), downcast a = Some v.
   Parameter downcast_elim: forall (a: t) T (v: T) (CAST: downcast a = Some v), (<<TY: (ty a) = T>>) /\ (<<VAL: (val a) ~= v>>).
   Parameter upcast_eta: forall (a: t), <<CAST: a = upcast (val a)>>.
+  Parameter upcast_elim: forall X (x: X), <<TY: ty (upcast x) = X>> /\ <<VAL: val (upcast x) ~= x>>.
   (* Parameter downcast_ty: forall (a: t), exists x, @downcast (ty a) a = Some x. *)
 
   (* Parameter patmat: forall R (body: forall (T: Type), T -> R), t -> R. *)
@@ -166,6 +169,76 @@ Module _Any: ANY.
     destruct a. refl.
   Qed.
 
+  Lemma upcast_elim: forall X (x: X), <<TY: ty (upcast x) = X>> /\ <<VAL: val (upcast x) ~= x>>.
+  Proof. i. ss. Qed.
+
+  Definition downcast_fst {T: Type} (a: t): option (T * t).
+    destruct a.
+    destruct (excluded_middle_informative (exists d, ty0 = (T * d)%type)).
+    - apply constructive_indefinite_description in e. destruct e. subst. destruct val0.
+      apply (Some (t0, upcast x)).
+    - apply None.
+  Defined.
+
+  Definition pair (a b: t): t := upcast (val a, val b).
+  Lemma type_pair_elim: forall (A B C: Type), (A * B)%type = (A * C)%type -> B = C.
+  Proof.
+    i.
+    assert(eq_JMeq: forall B (b0 b1: B) (eq: b0 = b1), b0 ~= b1).
+    { i; subst. refl. }
+    assert(apply_f: forall A B (a0 a1: A) (f: A -> B), a0 = a1 -> f a0 = f a1).
+    { ii; clarify. }
+    assert(prod_elim: forall A B (ab0 ab1: prod A B), ab0 = ab1 -> fst ab0 = fst ab1 /\ snd ab0 = snd ab1).
+    { destruct ab0, ab1; ss. i; clarify. }
+    Fail eapply prod_elim in H.
+    (* Set Printing All. *)
+    assert(T: (A * B)%type = (A * B)%type) by ss.
+    assert(U: (A * C)%type = (A * C)%type) by ss.
+    Fail eapply (apply_f) with (f:=fst) in T.
+    (* instantiate (1:=fst) in T. *)
+  Abort.
+
+  Inductive typrod {A B: Type}: Type :=
+  | typair: 
+
+  Lemma downcast_fst_spec
+        X (x: X) (a: t)
+    :
+      downcast_fst (pair (upcast x) a) = Some (x, a)
+  .
+  Proof.
+    unfold pair. unfold downcast_fst. des_ifs.
+    - des. unfold eq_rect_r.
+      unfold eq_rect in *.
+      unfold eq_sym. des_ifs.
+      f_equal. f_equal.
+      + assert(ty a = x0).
+        { destruct a; ss. clear - Heq.
+          unfold upcast in *.
+          (* Set Printing All. *)
+          injection Heq. i.
+          assert(eq_JMeq: forall B (b0 b1: B) (eq: b0 = b1), b0 ~= b1).
+          { i; subst. refl. }
+          (* assert(apply_f: forall A B (a0 a1: A) (f: A -> B), a0 ~= a1 -> f a0 = f a1). *)
+          assert(apply_f: forall A B (a0 a1: A) (f: A -> B), a0 = a1 -> f a0 = f a1).
+          { ii; clarify. }
+          assert(ty0 = x0).
+          { admit "somehow". }
+          exploit apply_f; try apply Heq.
+          Set Printing All.
+          rewrite H.
+          { instantiate (1:={| ty := X * ty0; val := (x, val0) |}). instantiate (1:={| ty := X * x0; val := (x1, x2) |}).
+            apply eq_JMeq. ss. }
+          instantiate (1:=fst).
+            apply JMeq_eq.
+            ss.
+          eapply JMeq_eq. Set Printing All. instantiate (1:=fst).
+          apply apply_f with (f:=fst) in Heq.
+          subst. clear - e. }
+        ss. unfold upcast in *. dependent destruction Heq.
+    -
+  Qed.
+
 End _Any.
 Goal _Any.upcast 0 = _Any.upcast () -> False. i. Fail injection H. Abort.
 
@@ -174,6 +247,46 @@ Goal _Any.upcast 0 = _Any.upcast () -> False. i. Fail injection H. Abort.
 Module Any.
   Include _Any.
   Definition pair (a b: Any.t): Any.t := Any.upcast (Any.val a, Any.val b).
+  
+  (* Definition downcast_fst {T: Type} (a: t): option (T * t). *)
+  (*   destruct a. *)
+  (*   destruct (excluded_middle_informative (exists d, ty0 = (T * d)%type)). *)
+  (*   - apply constructive_indefinite_description in e. destruct e. subst. destruct val0. *)
+  (*     apply (Some (t0, upcast x)). *)
+  (*   - apply None. *)
+  (* Defined. *)
+  Definition downcast_fst {T: Type} (a: t): option (T * t).
+    destruct (excluded_middle_informative (exists d, (Any.ty a) = (T * d)%type)).
+    - apply constructive_indefinite_description in e. destruct e. subst.
+      set (v:=val a). rewrite e in *. destruct v.
+      apply (Some (t0, upcast x0)).
+    - apply None.
+  Defined.
+
+  Lemma downcast_fst_spec
+        X (x: X) (a: Any.t)
+    :
+      downcast_fst (Any.pair (upcast x) a) = Some (x, a)
+  .
+  Proof.
+    unfold pair. unfold downcast_fst. des_ifs.
+    - des. f_equal.
+      unfold eq_rect in *.
+      destruct e0.
+      dependent destruction e0.
+
+      {
+      hexploit (upcast_elim x); et. i; des.
+      assert(eq_JMeq: forall B (b0 b1: B) (eq: b0 = b1), b0 ~= b1).
+      { i; subst. refl. }
+      exploit eq_JMeq; try apply e. intro P.
+      Unset Universe Checking.
+      rewrite VAL in P.
+      hexploit (upcast_elim (x, val a)); et. i; des.
+      rewrite TY0 in P. apply JMeq_eq in P. destruct P.
+      rewrite <- upcast_eta in *. assert(d = x0). { clear - e e0. rewrite e in *. clear - e0. remember (prod X d) as A. remember (prod X x0) as B. }
+  Qed.
+
 End Any.
 
 (* Notation "↑ a" := (Any.upcast a) (at level 60, only parsing). *)
